old/linearSearchAT.dfy
@@ -1,11 +1,25 @@
 include "../theory/math/SumReal.dfy"
 include "../theory/math/TypeR0.dfy"
 include "../theory/ComplexityR0.dfy"
-include "./linearSearch.dfy"
 
 import opened SumReal
 import opened TypeR0
 import opened ComplexityR0
+
+// Postcondition for a correct linear search algorithm
+ghost predicate post<A>(s:seq<A>, x:A, i:nat)
+{
+     (0 <= i < |s| ==> s[i] == x)
+  && (i == |s|     ==> (forall j :: 0 <= j < |s| ==> s[j] != x))
+}
+
+// Invariant for a correct linear search algorithm
+ghost predicate inv<A>(s:seq<A>, x:A, i:nat, n:nat)
+{
+     0 <= i <= n && n <= |s|
+  && (0 <= n < |s| ==> s[i] == x)      
+  && (n == |s|     ==> (forall j :: 0 <= j < i ==> s[j] != x))
+}
 
 ghost function T<A>(s:seq<A>, x:A, i:nat) : nat
   requires 0 <= i < |s|
@@ -22,18 +36,15 @@ ghost method linearSearchAT<A>(s:seq<A>, x:A) returns (i:nat, t:nat)
   ensures  exists k :: 0 <= k < |s| && s[k] == x && t == T(s, x, k)
 {
   var n:nat;
-  i, n, t := 0, |s|, 0;
-  while i != n
+  i, n, t := 0, |s|, 1;
+  while i != n && s[i] != x
     invariant inv(s, x, i, n)
-    invariant i <= n-1 ==> t == i    // =  T(|s|) - T(|s|-i)
-    invariant i == n   ==> t == i+1  // = (T(|s|) - T(|s|-i)) + 1
+    invariant forall j :: 0 <= j < i ==> s[j] != x
+    invariant exists k :: i <= k < |s| && s[k] == x
+    invariant t == i+1
     decreases n - i
   {
-    if s[i] != x {  // Op. interesante
-      i := i + 1 ;     
-    } else {
-      n := i;  // break;
-    }
+    i := i + 1;
     t := t + 1;
   }
   assert s[i] == x && t == T(s,x,i);
@@ -74,27 +85,27 @@ ghost method expectationLoop<A>(N:nat)
   assert bigO(Tavg, n => n as R0) by { var c, n0 := lem_TavgBigOlin(); }
 }
 
-ghost method inputScenario<A>(N:nat, p:nat) returns (s0:seq<A>, x0:A)
-  requires N > 0
-  requires 0 <= p < N
-  ensures  |s0| == N
-  ensures  forall i,j :: 0 <= i <= j < |s0| && i != j ==> s0[i] != s0[j]
-  ensures  s0[p] == x0
-{
-  assume {:axiom} 
-    exists s:seq<A> :: |s| == N && (forall i,j :: 0 <= i <= j < N && i != j ==> s[i] != s[j]);
-  s0 :| |s0| == N && forall i,j :: 0 <= i <= j < N && i != j ==> s0[i] != s0[j];
-  assume {:axiom} 
-    exists x:A :: s0[p] == x;
-  x0 :| s0[p] == x0;
-}
-
 ghost function probability<A>(s:seq<A>, x:A, p:nat) : R0
   requires 0 <= p < |s|
   requires s[p] == x
   requires forall i :: 0 <= i < |s| && i != p ==> s[i] != s[p]
 {
   1.0 / |s| as R0
+}
+
+ghost method inputScenario<A>(N:nat, p:nat) returns (s0:seq<A>, x0:A)
+  requires N > 0
+  requires 0 <= p < N
+  ensures  |s0| == N
+  ensures  s0[p] == x0
+  ensures  forall i :: 0 <= i < |s0| && i != p ==> s0[i] != s0[p]
+{
+  assume {:axiom} 
+    exists s:seq<A> :: |s| == N && (forall i :: 0 <= i < N && i != p ==> s[i] != s[p]);
+  s0 :| |s0| == N && forall i :: 0 <= i < N && i != p ==> s0[i] != s0[p];
+  assume {:axiom} 
+    exists x:A :: s0[p] == x;
+  x0 :| s0[p] == x0;
 }
 
 lemma lem_solveSum(N:nat)
