caseStudy/linearSearch.dfy
@@ -1,0 +1,50 @@
+
+/**************************************************************************
+  A correct linear search algorithm
+**************************************************************************/
+
+// Postcondition
+ghost predicate post<A>(s:seq<A>, x:A, i:nat)
+{
+     (0 <= i < |s| ==> s[i] == x)
+  && (i == |s|     ==> (forall j :: 0 <= j < |s| ==> s[j] != x))
+}
+
+// Invariant
+ghost predicate inv<A>(s:seq<A>, x:A, i:nat, n:nat)
+{
+     0 <= i <= n && n <= |s|
+  && (0 <= n < |s| ==> s[i] == x)      
+  && (n == |s|     ==> (forall j :: 0 <= j < i ==> s[j] != x))
+}
+
+method linearSearch<A(==)>(s:seq<A>, x:A) returns (i:nat)
+  ensures post(s, x, i)
+{
+  var n:nat;
+  i, n := 0, |s|;
+  while i != n
+    invariant inv(s, x, i, n)
+    decreases n - i
+  {
+    if s[i] != x {
+      i := i+1 ;     
+    } else {
+      n := i;  // break;
+    }
+  }
+} 
+
+// a more consize alternative
+method linearSearch2<A(==)>(s:seq<A>, x:A) returns (i:nat)
+  ensures post(s, x, i)
+{
+  var n:nat;
+  i, n := 0, |s|;
+  while i != n && s[i] != x
+    invariant inv(s, x, i, n)
+    decreases n - i
+  {
+    i := i + 1;
+  }
+} 
